io/case-studies/WebServer.fst
@@ -7,10 +7,9 @@ open DM.IIO.Tactics
 open Common
 open Types
 open DM
-open Model
 open Shared
 
-type plugin_type = ctx_s i m
+type plugin_type = Model.ctx_s i m
 
 (** since we do not have exceptions, we have to handle errors manually **)
 
@@ -20,8 +19,7 @@ let rec process_connections
   (plugin : plugin_type) : 
   IIO lfds pi
     (requires (fun _ -> True))
-    (ensures (fun _ _ _ -> True)) by (
-    explode (); bump_nth 34; iio_tactic ()) =
+    (ensures (fun _ _ _ -> True)) =
   match clients with
   | [] -> []
   | client :: tail -> begin
@@ -29,6 +27,7 @@ let rec process_connections
     if List.mem client to_read then begin
       let _ = plugin client in 
       let _ = static_cmd Close pi client in
+      lemma_append_enforced_locally pi;
       tail 
     end else clients
   end
@@ -53,7 +52,7 @@ let handle_connections
   (plugin : plugin_type) :
   IIO lfds m.pi 
     (requires (fun _ -> True))
-    (ensures (fun _ _ _ -> True)) by (iio_tactic ()) =
+    (ensures (fun _ _ _ -> True)) =
   match static_cmd Select pi (clients, [], [], 100uy) with
   | Inl (to_read, _, _) ->
     let clients'' = process_connections clients to_read plugin in
@@ -66,7 +65,8 @@ let server_loop_body
   (clients : lfds) :
   IIO lfds m.pi
     (requires (fun h -> True)) 
-    (ensures (fun h r lt -> True)) by (iio_tactic ()) = 
+    (ensures (fun h r lt -> True)) = 
+  lemma_append_enforced_locally m.pi;
   let clients' = (match get_new_connection socket with
                  | None -> clients
                  | Some fd -> fd :: clients) in
@@ -79,7 +79,8 @@ let rec server_loop
   (clients : lfds) :
   IIO unit m.pi
     (requires (fun h -> True))
-    (ensures (fun h r lt -> True)) by (explode (); bump_nth 18; iio_tactic ()) =
+    (ensures (fun h r lt -> True)) =
+  lemma_append_enforced_locally m.pi;
   if iterations_count = 0 then ()
   else begin
     let clients' = server_loop_body socket plugin clients in
@@ -92,13 +93,14 @@ let create_basic_server (ip:string) (port:UInt8.t) (limit:UInt8.t) :
     (ensures (fun h r lt ->
       match r with
       | Inl socket -> is_open socket (apply_changes h lt)
-      | _ -> True)) by (explode ()) =
+      | _ -> True)) by (explode ()) = 
   match static_cmd Socket pi () with
   | Inl socket -> 
     let _ = static_cmd Setsockopt pi (socket, SO_REUSEADDR, true) in 
     let _ = static_cmd Bind pi (socket, ip, port) in
     let _ = static_cmd Listen pi (socket, limit) in
     let _ = static_cmd SetNonblock pi socket in
+    lemma_append_enforced_locally m.pi;
     Inl socket 
   | Inr err -> Inr err
 
@@ -106,7 +108,8 @@ let webserver
   (plugin : plugin_type) :
   IIO i.ret m.pi
     (requires (fun h -> True))
-    (ensures (fun h r lt -> True)) by (explode (); bump_nth 11; iio_tactic ()) =
+    (ensures (fun h r lt -> True)) by (explode ()) =
+  lemma_append_enforced_locally m.pi;
   match create_basic_server "0.0.0.0" 81uy 5uy with
   | Inl server -> begin
       server_loop 100000000000 server plugin []
